src/program_logic/crash_adequacy.v
@@ -33,6 +33,7 @@ Lemma wpc_step s e1 σ1 g1 ns D κ κs e2 σ2 g2 efs m Φ Φc :
   state_interp σ1 m -∗
   global_state_interp g1 ns mj D (κ ++ κs) -∗
   WPC e1 @ s; ⊤ {{ Φ }} {{ Φc }} -∗ NC 1 -∗
+  £ (S $ num_laters_per_step ns) -∗
   ||={⊤|⊤,∅|∅}=> ||▷=>^(S $ num_laters_per_step ns) ||={∅|∅,⊤|⊤}=>
   state_interp σ2 (length efs + m) ∗
   global_state_interp g2 (step_count_next ns) mj D κs ∗
@@ -40,11 +41,11 @@ Lemma wpc_step s e1 σ1 g1 ns D κ κs e2 σ2 g2 efs m Φ Φc :
   wptp s efs ∗
   NC 1.
 Proof.
-  rewrite {1}wpc0_unfold /wpc_pre. iIntros (?) "Hσ Hg H HNC".
+  rewrite {1}wpc0_unfold /wpc_pre. iIntros (?) "Hσ Hg H HNC Hlc".
   rewrite (val_stuck e1 σ1 g1 κ e2 σ2 g2 efs) //.
   iDestruct "H" as "(H&_)".
   iMod (fupd2_mask_subseteq ⊤ (⊤ ∖ D)) as "Hclo"; try set_solver+.
-  iMod ("H" $! _ σ1 with "Hσ Hg HNC") as "H".
+  iMod ("H" $! _ σ1 with "Hσ Hg HNC Hlc") as "H".
   iModIntro.
   iApply (step_fupd2N_wand with "H"). iIntros "(_&H)".
   iMod ("H" $! e2 σ2 g2 efs with "[//]") as "H".
@@ -56,22 +57,23 @@ Lemma wptp_step s e1 t1 t2 κ κs σ1 g1 ns D σ2 g2 Φ Φc :
   step (e1 :: t1,(σ1,g1)) κ (t2, (σ2,g2)) →
   state_interp σ1 (length t1) -∗
   global_state_interp g1 ns mj D (κ ++ κs) -∗
-  WPC e1 @ s; ⊤ {{ Φ }} {{ Φc }}-∗ wptp s t1 -∗ NC 1 ==∗
+  WPC e1 @ s; ⊤ {{ Φ }} {{ Φc }}-∗ wptp s t1 -∗ NC 1 -∗
+  £ (S $ num_laters_per_step ns) ==∗
   ∃ e2 t2', ⌜t2 = e2 :: t2'⌝ ∗
   ||={⊤|⊤,∅|∅}=> ||▷=>^(S $ num_laters_per_step ns) ||={∅|∅,⊤|⊤}=>
   state_interp σ2 (pred (length t2)) ∗
   global_state_interp g2 (step_count_next ns) mj D κs ∗
   WPC e2 @ s; ⊤ {{ Φ }} {{ Φc}} ∗ wptp s t2' ∗ NC 1.
 Proof.
-  iIntros (Hstep) "Hσ Hg He Ht HNC".
+  iIntros (Hstep) "Hσ Hg He Ht HNC Hlc".
   destruct Hstep as [e1' σ1' g1' e2' σ2' g2' efs [|? t1'] t2' ?? Hstep]; simplify_eq/=.
   - iExists e2', (t2' ++ efs). iModIntro. iSplitR; first by eauto.
-    iMod (wpc_step with "Hσ Hg He HNC") as "H"; first done. iModIntro.
+    iMod (wpc_step with "Hσ Hg He HNC Hlc") as "H"; first done. iModIntro.
     iApply (step_fupd2N_wand with "H"). iIntros ">(Hσ & Hg & He2 & Hefs) !>".
     rewrite Nat.add_comm app_length. by iFrame.
   - iExists e, (t1' ++ e2' :: t2' ++ efs); iSplitR; first eauto.
     iDestruct "Ht" as "(Ht1 & He1 & Ht2)".
-    iModIntro. iMod (wpc_step with "Hσ Hg He1 HNC") as "H"; first done. iModIntro.
+    iModIntro. iMod (wpc_step with "Hσ Hg He1 HNC Hlc") as "H"; first done. iModIntro.
     iApply (step_fupd2N_wand with "H"). iIntros ">(Hσ & Hg & He2 & Hefs) !>".
     rewrite !app_length /= !app_length.
     replace (length t1' + S (length t2' + length efs))
@@ -108,6 +110,7 @@ Lemma wptp_steps s n e1 t1 κs κs' t2 σ1 g1 ns D σ2 g2 Φ Φc :
   state_interp σ1 (length t1) -∗
   global_state_interp g1 ns mj D (κs ++ κs') -∗
   WPC e1 @ s; ⊤ {{ Φ }} {{ Φc }} -∗ wptp s t1 -∗ NC 1 -∗
+  £ (steps_sum num_laters_per_step step_count_next ns n) -∗
   (||={⊤|⊤, ∅|∅}=> ||▷=>^(steps_sum num_laters_per_step step_count_next ns n) ||={∅|∅,⊤|⊤}=> ∃ e2 t2',
     ⌜t2 = e2 :: t2'⌝ ∗
     state_interp σ2 (pred (length t2)) ∗
@@ -117,16 +120,18 @@ Lemma wptp_steps s n e1 t1 κs κs' t2 σ1 g1 ns D σ2 g2 Φ Φc :
 Proof.
   revert e1 t1 κs κs' t2 σ1 g1 ns σ2 g2; simpl.
   induction n as [|n IH]=> e1 t1 κs κs' t2 σ1 g1 ns σ2 g2 /=.
-  { inversion_clear 1; iIntros "?????"; iExists e1, t1; iFrame; eauto 10.
+  { inversion_clear 1; iIntros "??????"; iExists e1, t1; iFrame; eauto 10.
     iApply fupd2_mask_intro_subseteq; eauto. }
-  iIntros (Hsteps) "Hσ Hg He Ht HNC". inversion_clear Hsteps as [|?? [t1' [σ1' g1']]].
+  iIntros (Hsteps) "Hσ Hg He Ht HNC Hlc". inversion_clear Hsteps as [|?? [t1' [σ1' g1']]].
   rewrite -(assoc_L (++)).
+  rewrite -Nat.add_succ_l lc_split.
+  iDestruct "Hlc" as "[Hlc1 Hlc2]".
   iApply step_fupd2N_inner_plus.
-  iMod (wptp_step with "Hσ Hg He Ht HNC") as (e1' t1'' ?) ">H"; first eauto; simplify_eq.
+  iMod (wptp_step with "Hσ Hg He Ht HNC Hlc1") as (e1' t1'' ?) ">H"; first eauto; simplify_eq.
   iApply (step_fupd2N_wand with "H"). iIntros "!> H".
   iMod "H".
   iDestruct "H" as "(Hσ & Hg & He & Ht & HNC)".
-  iMod (IH with "Hσ Hg He Ht HNC") as "IH"; first done.
+  iMod (IH with "Hσ Hg He Ht HNC Hlc2") as "IH"; first done.
   rewrite -Nat_iter_S_r.
   iModIntro. iModIntro. eauto.
 Qed.
@@ -135,16 +140,17 @@ Lemma wpc_safe κs m e σ g ns D Φ Φc q :
   state_interp σ m -∗
   global_state_interp g ns mj D κs -∗
   WPC e @ ⊤ {{ Φ }} {{ Φc }} -∗ NC q -∗
+  £ (S $ num_laters_per_step ns) -∗
   ||={⊤|⊤, ∅|∅}=> ||▷=>^(num_laters_per_step ns + 1)
   ⌜is_Some (to_val e) ∨ reducible e σ g⌝.
 Proof.
   rewrite wpc0_unfold /wpc_pre. iIntros "Hσ Hg H". iDestruct "H" as "(H&_)".
   destruct (to_val e) as [v|] eqn:?.
-  { iIntros "_". iApply fupd2_mask_intro; [done..|].
+  { iIntros "_ _". iApply fupd2_mask_intro; [done..|].
     iIntros "_". iApply step_fupd2N_later. auto. }
-  iIntros "HNC".
+  iIntros "HNC Hlc".
   iMod (fupd2_mask_subseteq ⊤ (⊤ ∖ D)) as "Hclo"; try set_solver+.
-  iMod ("H" $! _ _ _ _ _ [] with "[$] [$] [$]") as "H".
+  iMod ("H" $! _ _ _ _ _ [] with "[$] [$] [$] [$]") as "H".
   simpl. iModIntro. rewrite [_ + 1]comm. iApply (step_fupd2N_wand with "H").
   iNext. iIntros "(%Hred&Hclo')". eauto.
 Qed.
@@ -156,6 +162,7 @@ Local Lemma wptp0_strong_adequacy Φ Φc κs' s n e1 t1 κs t2 σ1 g1 ns D σ2 g
   WPC e1 @ s; ⊤ {{ Φ }} {{ Φc }} -∗
   wptp s t1 -∗
   NC 1 -∗
+  £ (steps_sum num_laters_per_step step_count_next ns n) -∗
   ||={⊤|⊤,∅|∅}=> ||▷=>^(steps_sum num_laters_per_step step_count_next ns n) ||={∅|∅, ⊤|⊤}=> (∃ e2 t2',
     ⌜ t2 = e2 :: t2' ⌝ ∗
     state_interp σ2 (length t2') ∗
@@ -164,8 +171,8 @@ Local Lemma wptp0_strong_adequacy Φ Φc κs' s n e1 t1 κs t2 σ1 g1 ns D σ2 g
     ([∗ list] v ∈ omap to_val t2', fork_post v) ∗
     NC 1).
 Proof.
-  iIntros (Hstep) "Hσ Hg He Ht HNC".
-  iMod (wptp_steps with "Hσ Hg He Ht HNC") as "Hwp"; first done.
+  iIntros (Hstep) "Hσ Hg He Ht HNC Hlc".
+  iMod (wptp_steps with "Hσ Hg He Ht HNC Hlc") as "Hwp"; first done.
   iModIntro. iApply (step_fupd2N_wand with "Hwp").
   iMod 1 as (e2' t2' ?) "(Hσ & Hg & Hwp & Ht & HNC)"; simplify_eq/=.
   iExists _, _. iSplitL ""; first done. iFrame "Hσ".
@@ -190,20 +197,23 @@ Local Lemma wptp0_progress Φ Φc κs' n e1 t1 κs t2 σ1 g1 ns D σ2 g2 e2 :
   WPC e1 @ NotStuck; ⊤ {{ Φ }} {{ Φc }} -∗
   wptp NotStuck t1 -∗
   NC 1 -∗
+  £ (steps_sum num_laters_per_step step_count_next ns (S n)) -∗
   ||={⊤|⊤,∅|∅}=> ||▷=>^(steps_sum num_laters_per_step step_count_next ns n) ||={∅|∅, ∅|∅}=>
   ||▷=>^(num_laters_per_step (Nat.iter n step_count_next ns) + 1)
    ⌜ not_stuck e2 σ2 g2 ⌝.
 Proof.
-  iIntros (Hstep Hel) "Hσ Hg He Ht HNC".
-  iMod (wptp_steps with "Hσ Hg He Ht HNC") as "Hwp"; first done.
+  iIntros (Hstep Hel) "Hσ Hg He Ht HNC Hlc".
+  rewrite steps_sum_S_r.
+  iDestruct "Hlc" as "[Hlc1 Hlc2]".
+  iMod (wptp_steps with "Hσ Hg He Ht HNC Hlc1") as "Hwp"; first done.
   iModIntro. iApply (step_fupd2N_wand with "Hwp").
   iMod 1 as (e2' t2' ?) "(Hσ & Hg & Hwp & Ht & HNC)"; simplify_eq/=.
   apply elem_of_cons in Hel as [<-|(t1''&t2''&->)%elem_of_list_split].
-  - iPoseProof (wpc_safe with "Hσ Hg Hwp") as "H".
-    iMod ("H" with "[$]") as "H"; eauto.
+  - iPoseProof (wpc_safe with "Hσ Hg Hwp HNC Hlc2") as "H".
+    iMod "H". eauto.
   - iDestruct "Ht" as "(_ & He' & _)".
-    iPoseProof (wpc_safe with "Hσ Hg He'") as "H".
-    by iMod ("H" with "[$]") as "H".
+    iPoseProof (wpc_safe with "Hσ Hg He' HNC Hlc2") as "H".
+    by iMod "H".
 Qed.
 
 Local Lemma wptp0_strong_crash_adequacy Φ Φc κs' s n e1 t1 κs t2 σ1 g1 ns D σ2 g2 :
@@ -213,14 +223,18 @@ Local Lemma wptp0_strong_crash_adequacy Φ Φc κs' s n e1 t1 κs t2 σ1 g1 ns D
   WPC e1 @ s; ⊤ {{ Φ }} {{ Φc }} -∗
   wptp s t1 -∗
   NC 1 -∗
+  £ (steps_sum num_laters_per_step step_count_next ns (S n)) -∗
   ||={⊤|⊤,∅|∅}=> ||▷=>^(steps_sum num_laters_per_step step_count_next ns (S n)) ||={∅|∅, ⊤|⊤}=>
   ▷ (∃ e2 t2',
     ⌜ t2 = e2 :: t2' ⌝ ∗
     Φc ∗ state_interp σ2 (length t2') ∗ global_state_interp g2 ((Nat.iter n step_count_next ns)) mj D κs' ∗ C).
 Proof.
-  iIntros (Hstep) "Hσ Hg He Ht HNC".
-  iDestruct (wptp_steps with "Hσ Hg He Ht HNC") as "Hwp"; first done.
+  iIntros (Hstep) "Hσ Hg He Ht HNC Hlc".
   rewrite steps_sum_S_r.
+  iDestruct "Hlc" as "[Hlc1 Hlc2]".
+  (* We are not even using Hlc2, but it is probably better to keep the credits and laters
+     in sync in the lemma statement. *)
+  iDestruct (wptp_steps with "Hσ Hg He Ht HNC Hlc1") as "Hwp"; first done.
   iApply step_fupd2N_inner_plus.
   iApply (step_fupd2N_inner_wand with "Hwp"); auto.
   iDestruct 1 as (e2' t2' ?) "(Hσ & Hg & Hwp & Ht & HNC)"; simplify_eq/=.
@@ -253,6 +267,7 @@ Lemma wptp_strong_adequacy Φ Φc κs' s n e1 t1 κs t2 σ1 g1 ns mj D σ2 g2 :
   WPC e1 @ s; ⊤ {{ Φ }} {{ Φc }} -∗
   wptp s t1 -∗
   NC 1 -∗
+  £ (steps_sum num_laters_per_step step_count_next ns n) -∗
   ||={⊤|⊤,∅|∅}=> ||▷=>^(steps_sum num_laters_per_step step_count_next ns n) ||={∅|∅, ⊤|⊤}=> (∃ e2 t2',
     ⌜ t2 = e2 :: t2' ⌝ ∗
     state_interp σ2 (length t2') ∗
@@ -261,8 +276,8 @@ Lemma wptp_strong_adequacy Φ Φc κs' s n e1 t1 κs t2 σ1 g1 ns mj D σ2 g2 :
     ([∗ list] v ∈ omap to_val t2', fork_post v) ∗
     NC 1).
 Proof.
-  iIntros (?) "?? Hwpc Hwptp Hnc".
-  iApply (wptp0_strong_adequacy mj with "[$] [$] [Hwpc] [Hwptp] [$]"); first eassumption.
+  iIntros (?) "?? Hwpc Hwptp Hnc Hlc".
+  iApply (wptp0_strong_adequacy mj with "[$] [$] [Hwpc] [Hwptp] [$] [$]"); first eassumption.
   { by iApply wpc0_wpc. }
   { iApply (big_sepL_mono with "Hwptp"). iIntros.
     iApply (wpc0_wpc); eauto.
@@ -277,12 +292,13 @@ Lemma wptp_progress Φ Φc κs' n e1 t1 κs t2 σ1 g1 ns mj D σ2 g2 e2 :
   WPC e1 @ NotStuck; ⊤ {{ Φ }} {{ Φc }} -∗
   wptp NotStuck t1 -∗
   NC 1 -∗
+  £ (steps_sum num_laters_per_step step_count_next ns (S n)) -∗
   ||={⊤|⊤,∅|∅}=> ||▷=>^(steps_sum num_laters_per_step step_count_next ns n) ||={∅|∅, ∅|∅}=>
   ||▷=>^(num_laters_per_step (Nat.iter n step_count_next ns) + 1)
   (⌜not_stuck e2 σ2 g2 ⌝).
 Proof.
-  iIntros (??) "?? Hwpc Hwptp Hnc".
-  iApply (wptp0_progress mj with "[$] [$] [Hwpc] [Hwptp] [$]"); first done; first done.
+  iIntros (??) "?? Hwpc Hwptp Hnc Hlc".
+  iApply (wptp0_progress mj with "[$] [$] [Hwpc] [Hwptp] [$] [$]"); first done; first done.
   { by iApply wpc0_wpc. }
   { iApply (big_sepL_mono with "Hwptp"). iIntros.
     iApply (wpc0_wpc); eauto.
@@ -296,13 +312,14 @@ Lemma wptp_strong_crash_adequacy Φ Φc κs' s n e1 t1 κs t2 σ1 g1 ns mj D σ2
   WPC e1 @ s; ⊤ {{ Φ }} {{ Φc }} -∗
   wptp s t1 -∗
   NC 1 -∗
+  £ (steps_sum num_laters_per_step step_count_next ns (S n)) -∗
   ||={⊤|⊤,∅|∅}=> ||▷=>^(steps_sum num_laters_per_step step_count_next ns (S n)) ||={∅|∅, ⊤|⊤}=>
   ▷ (∃ e2 t2',
     ⌜ t2 = e2 :: t2' ⌝ ∗
     Φc ∗ state_interp σ2 (length t2') ∗ global_state_interp g2 (Nat.iter n step_count_next ns) mj D κs' ∗ C).
 Proof.
-  iIntros (?) "?? Hwpc Hwptp Hnc".
-  iApply (wptp0_strong_crash_adequacy mj with "[$] [$] [Hwpc] [Hwptp] [$]"); first eassumption.
+  iIntros (?) "?? Hwpc Hwptp Hnc Hlc".
+  iApply (wptp0_strong_crash_adequacy mj with "[$] [$] [Hwpc] [Hwptp] [$] Hlc"); first eassumption.
   { by iApply wpc0_wpc. }
   { iApply (big_sepL_mono with "Hwptp"). iIntros.
     iApply (wpc0_wpc); eauto.
